src/NLustre/NLSemantics.v
@@ -86,9 +86,7 @@ Module Type NLSEMANTICS
     with sem_reset: ident -> stream bool -> stream (list value) -> stream (list value) -> Prop :=
          | SReset:
              forall f r xss yss,
-               (forall k, sem_node f
-                              (mask (all_absent (xss 0)) k r xss)
-                              (mask (all_absent (yss 0)) k r yss)) ->
+               (forall k, sem_node f (mask_v k r xss) (mask_v k r yss)) ->
                sem_reset f r xss yss
 
     with sem_node: ident -> stream (list value) -> stream (list value) -> Prop :=
@@ -239,12 +237,8 @@ enough: it does not support the internal fixpoint introduced by
 
     Hypothesis ResetCase:
       forall f r xss yss,
-        (forall k, sem_node G f
-                       (mask (all_absent (xss 0)) k r xss)
-                       (mask (all_absent (yss 0)) k r yss)
-              /\ P_node f
-                       (mask (all_absent (xss 0)) k r xss)
-                       (mask (all_absent (yss 0)) k r yss)) ->
+        (forall k, sem_node G f (mask_v k r xss) (mask_v k r yss)
+              /\ P_node f (mask_v k r xss) (mask_v k r yss)) ->
         P_reset f r xss yss.
 
     Hypothesis NodeCase:
@@ -542,8 +536,9 @@ enough: it does not support the internal fixpoint introduced by
     intros * E1 ? ? E2 ? ? E3 Res.
     inversion_clear Res as [? ? ? ? Node].
     constructor; intro k.
-
-    specialize (Node k). now rewrite <-E1, <-2 E2, <-2 E3.
+    specialize (Node k).
+    unfold mask_v in *.
+    now rewrite <-E1, <-2 E2, <-2 E3.
   Qed.
 
 End NLSEMANTICS.
